Effect: add other effect_kind

experiment/Experiment.Steel.Combinators.fst
@@ -2,6 +2,7 @@ module Experiment.Steel.Combinators
 
 module U   = Learn.Util
 module L   = FStar.List.Pure
+module T   = FStar.Tactics
 module SE  = Steel.Effect
 module SH  = Experiment.Steel.Steel
 module Fl  = Learn.FList
@@ -162,6 +163,17 @@ let return_steel
     Steel.Effect.Atomic.return x)
 
 inline_for_extraction noextract
+let return_ghostI_steel
+      (a : Type) (opened : Mem.inames) (x : a) (sl_hint : post_t a)
+      (pre : pre_t) (post : post_t a)
+      (e : Veq.vequiv pre (post x))
+  : (let c = TCret #a #x #sl_hint pre post e in
+     repr_steel_t (SH.KGhostI opened) a pre post (tree_req _ c) (tree_ens _ c))
+  = SH.ghostI_f #opened (fun () ->
+    (**) e.veq_g _;
+    Steel.Effect.Atomic.return x)
+
+inline_for_extraction noextract
 let return_ghost_steel
       (a : Type) (opened : Mem.inames) (x : a) (sl_hint : post_t a)
       (pre : pre_t) (post : post_t a)
@@ -171,6 +183,7 @@ let return_ghost_steel
   = SH.ghost_f #opened (fun () ->
     (**) e.veq_g _;
     x)
+
 
 [@@ __repr_M__]
 inline_for_extraction noextract
@@ -185,8 +198,14 @@ let return_hint (#a : Type) (x : a) (sl_hint : post_t a)
 
 [@@ __repr_M__]
 inline_for_extraction noextract
-let return (#a : Type) (x : a) : repr SH.KSteel a
-  = return_hint x (fun _ -> [])
+let return_ghostI_hint (#a : Type) (#opened : Mem.inames) (x : a) (sl_hint : post_t a)
+  : repr (SH.KGhostI opened) a
+  = {
+    repr_tree  = Tret a x sl_hint;
+    repr_steel = (fun pre0 post0 c ->
+        let TCret pre post p = c in
+        return_ghostI_steel a opened x sl_hint pre post p)
+  }
 
 [@@ __repr_M__]
 inline_for_extraction noextract
@@ -198,6 +217,11 @@ let return_ghost_hint (#a : Type) (#opened : Mem.inames) (x : a) (sl_hint : post
         let TCret pre post p = c in
         return_ghost_steel a opened x sl_hint pre post p)
   }
+
+[@@ __repr_M__]
+inline_for_extraction noextract
+let return (#a : Type) (x : a) : repr SH.KSteel a
+  = return_hint x (fun _ -> [])
 
 [@@ __repr_M__]
 inline_for_extraction noextract
@@ -258,6 +282,69 @@ let bind_steel
 
 [@@FStar.Tactics.(postprocess_with (fun () -> norm __postprocess_steps; trefl ()))]
 inline_for_extraction noextract
+let bind_atomic_ghost_steel
+      (a : Type) (b : Type) (opened : Mem.inames) (f : prog_tree a) (g : (a -> prog_tree b))
+      (pre : pre_t) (itm : post_t a) (post : post_t b)
+      (cf : tree_cond f pre itm) (cg : ((x : a) -> tree_cond (g x) (itm x) post))
+      ($rf : repr_steel_t (SH.KAtomic opened) a pre itm (tree_req f cf) (tree_ens f cf))
+      ($rg : (x : a) ->
+             repr_steel_t (SH.KGhostI opened) b (itm x) post (tree_req (g x) (cg x)) (tree_ens (g x) (cg x)))
+  : (let c = TCbind #a #b #f #g pre itm post cf cg in
+     repr_steel_t (SH.KAtomic opened) b pre post (tree_req _ c) (tree_ens _ c))
+  = SH.atomic_f (fun () ->
+    (**) let sl0 = gget (vprop_of_list pre) in
+    (**) (elim_tree_req_bind f g cf cg sl0; ());
+    let x = SH.atomic_u rf () in
+    (**) let sl1 = gget (vprop_of_list (itm x)) in
+    let y = SH.ghostI_u (rg x) () in
+    (**) let sl2 = gget (vprop_of_list (post y)) in
+    (**) (intro_tree_ens_bind f g cf cg sl0 x sl1 y sl2; ());
+    Steel.Effect.Atomic.return y)
+
+[@@FStar.Tactics.(postprocess_with (fun () -> norm __postprocess_steps; trefl ()))]
+inline_for_extraction noextract
+let bind_ghost_atomic_steel
+      (a : Type) (b : Type) (opened : Mem.inames) (f : prog_tree a) (g : (a -> prog_tree b))
+      (pre : pre_t) (itm : post_t a) (post : post_t b)
+      (cf : tree_cond f pre itm) (cg : ((x : a) -> tree_cond (g x) (itm x) post))
+      ($rf : repr_steel_t (SH.KGhostI opened) a pre itm (tree_req f cf) (tree_ens f cf))
+      ($rg : (x : a) ->
+             repr_steel_t (SH.KAtomic opened) b (itm x) post (tree_req (g x) (cg x)) (tree_ens (g x) (cg x)))
+  : (let c = TCbind #a #b #f #g pre itm post cf cg in
+     repr_steel_t (SH.KAtomic opened) b pre post (tree_req _ c) (tree_ens _ c))
+  = SH.atomic_f (fun () ->
+    (**) let sl0 = gget (vprop_of_list pre) in
+    (**) (elim_tree_req_bind f g cf cg sl0; ());
+    let x = SH.ghostI_u rf () in
+    (**) let sl1 = gget (vprop_of_list (itm x)) in
+    let y = SH.atomic_u (rg x) () in
+    (**) let sl2 = gget (vprop_of_list (post y)) in
+    (**) (intro_tree_ens_bind f g cf cg sl0 x sl1 y sl2; ());
+    Steel.Effect.Atomic.return y)
+
+[@@FStar.Tactics.(postprocess_with (fun () -> norm __postprocess_steps; trefl ()))]
+inline_for_extraction noextract
+let bind_ghostI_steel
+      (a : Type) (b : Type) (opened : Mem.inames) (f : prog_tree a) (g : (a -> prog_tree b))
+      (pre : pre_t) (itm : post_t a) (post : post_t b)
+      (cf : tree_cond f pre itm) (cg : ((x : a) -> tree_cond (g x) (itm x) post))
+      ($rf : repr_steel_t (SH.KGhostI opened) a pre itm (tree_req f cf) (tree_ens f cf))
+      ($rg : (x : a) ->
+             repr_steel_t (SH.KGhostI opened) b (itm x) post (tree_req (g x) (cg x)) (tree_ens (g x) (cg x)))
+  : (let c = TCbind #a #b #f #g pre itm post cf cg in
+     repr_steel_t (SH.KGhostI opened) b pre post (tree_req _ c) (tree_ens _ c))
+  = SH.ghostI_f #opened (fun () ->
+    (**) let sl0 = gget (vprop_of_list pre) in
+    (**) (elim_tree_req_bind f g cf cg sl0; ());
+    let x = SH.ghostI_u rf () in
+    (**) let sl1 = gget (vprop_of_list (itm x)) in
+    let y = SH.ghostI_u (rg x) () in
+    (**) let sl2 = gget (vprop_of_list (post y)) in
+    (**) (intro_tree_ens_bind f g cf cg sl0 x sl1 y sl2; ());
+    Steel.Effect.Atomic.return y)
+
+[@@FStar.Tactics.(postprocess_with (fun () -> norm __postprocess_steps; trefl ()))]
+inline_for_extraction noextract
 let bind_ghost_steel
       (a : Type) (b : Type) (opened : Mem.inames) (f : prog_tree a) (g : (a -> prog_tree b))
       (pre : pre_t) (itm : post_t a) (post : post_t b)
@@ -280,31 +367,41 @@ let bind_ghost_steel
 
 [@@ __repr_M__]
 inline_for_extraction noextract
-let bind (#a #b : Type) (f : repr SH.KSteel a) (g : a -> repr SH.KSteel b)
-  : repr SH.KSteel b
+let bind_ek (#a #b : Type) (ek0 ek1 ek2 : SH.effect_kind)
+      (s : (a : Type) -> (b : Type) -> (f : prog_tree a) -> (g : (a -> prog_tree b)) ->
+           (pre : pre_t) -> (itm : post_t a) -> (post : post_t b) ->
+           (cf : tree_cond f pre itm) -> (cg : ((x : a) -> tree_cond (g x) (itm x) post)) ->
+           (rf : repr_steel_t ek0 a pre itm (tree_req f cf) (tree_ens f cf)) ->
+           (rg : ((x : a) -> repr_steel_t ek1 b (itm x) post (tree_req (g x) (cg x)) (tree_ens (g x) (cg x)))) ->
+           (let c = TCbind #a #b #f #g pre itm post cf cg in
+            repr_steel_t ek2 b pre post (tree_req _ c) (tree_ens _ c)))
+      (f : repr ek0 a) (g : a -> repr ek1 b)
+  : repr ek2 b
   = {
     repr_tree  = Tbind a b f.repr_tree (fun x -> (g x).repr_tree);
     repr_steel = (fun pre0 post0 c ->
                     let (TCbind #a' #b' #tf #tg pre itm post cf cg) = c in
-                    let rg (x : a) : repr_steel_t SH.KSteel b (itm x) post _ _
+                    let rg (x : a) : repr_steel_t ek1 b (itm x) post _ _
                                    = (g x).repr_steel _ _ (cg x) in
-                    bind_steel a b tf tg pre itm post cf cg (f.repr_steel _ _ cf) rg)
+                    s a b tf tg pre itm post cf cg (f.repr_steel _ _ cf) rg)
   }
+
+[@@ __repr_M__]
+inline_for_extraction noextract
+let bind (#a #b : Type) (f : repr SH.KSteel a) (g : a -> repr SH.KSteel b)
+  : repr SH.KSteel b
+  = bind_ek SH.KSteel SH.KSteel SH.KSteel
+      (fun a b f g pre itm post cf cg rf rg -> bind_steel a b f g pre itm post cf cg rf rg)
+      f g
 
 [@@ __repr_M__]
 inline_for_extraction noextract
 let bind_ghost (#a #b : Type) (#opened : Mem.inames)
                (f : repr (SH.KGhost opened) a) (g : a -> repr (SH.KGhost opened) b)
   : repr (SH.KGhost opened) b
-  = {
-    repr_tree  = Tbind a b f.repr_tree (fun x -> (g x).repr_tree);
-    repr_steel = (fun pre0 post0 c ->
-                    let (TCbind #a' #b' #tf #tg pre itm post cf cg) = c in
-                    let rg (x : a) : repr_steel_t (SH.KGhost opened) b (itm x) post _ _
-                                   = (g x).repr_steel _ _ (cg x) in
-                    bind_ghost_steel a b opened tf tg pre itm post cf cg (f.repr_steel _ _ cf) rg)
-  }
-
+  = bind_ek (SH.KGhost opened) (SH.KGhost opened) (SH.KGhost opened)
+      (fun a b f g pre itm post cf cg rf rg -> bind_ghost_steel a b opened f g pre itm post cf cg rf rg)
+      f g
 
 
 (****** Bind pure *)
@@ -314,7 +411,7 @@ let bindP_steel
       (a : Type) (b : Type) (wp : pure_wp a) ($f : unit -> PURE a wp) (g : (a -> prog_tree b))
       (pre : pre_t) (post : post_t b)
       (cg : ((x : a) -> tree_cond (g x) pre post))
-      ($rg : (x : a) -> repr_steel_t SH.KSteel b pre post (tree_req (g x) (cg x)) (tree_ens (g x) (cg x)))
+      (rg : (x : a) -> repr_steel_t SH.KSteel b pre post (tree_req (g x) (cg x)) (tree_ens (g x) (cg x)))
   : (let c = TCbindP #a #b #wp #g pre post cg in
      repr_steel_t SH.KSteel b pre post (tree_req _ c) (tree_ens _ c))
   = 
@@ -324,11 +421,39 @@ let bindP_steel
     SH.steel_u (rg x) ())
 
 inline_for_extraction noextract
-let bindP_ghost_steel
-      (a : Type) (b : Type) (opened : Mem.inames) (wp : pure_wp a) ($f : unit -> GHOST a wp) (g : (a -> prog_tree b))
+let bindP_atomic_steel
+      (a : Type) (b : Type) (opened : Mem.inames) (wp : pure_wp a) ($f : unit -> PURE a wp) (g : (a -> prog_tree b))
       (pre : pre_t) (post : post_t b)
       (cg : ((x : a) -> tree_cond (g x) pre post))
-      ($rg : (x : a) -> repr_steel_t (SH.KGhost opened) b pre post (tree_req (g x) (cg x)) (tree_ens (g x) (cg x)))
+      (rg : (x : a) -> repr_steel_t (SH.KAtomic opened)  b pre post (tree_req (g x) (cg x)) (tree_ens (g x) (cg x)))
+  : (let c = TCbindP #a #b #wp #g pre post cg in
+     repr_steel_t (SH.KAtomic opened) b pre post (tree_req _ c) (tree_ens _ c))
+  = 
+    FStar.Monotonic.Pure.elim_pure_wp_monotonicity wp;
+    SH.atomic_f (fun () ->
+    let x = f () in
+    SH.atomic_u (rg x) ())
+
+inline_for_extraction noextract
+let bindP_ghostI_steel
+      (a : Type) (b : Type) (opened : Mem.inames) (wp : pure_wp a) ($f : unit -> PURE a wp) (g : (a -> prog_tree b))
+      (pre : pre_t) (post : post_t b)
+      (cg : ((x : a) -> tree_cond (g x) pre post))
+      ($rg : (x : a) -> repr_steel_t (SH.KGhostI opened)  b pre post (tree_req (g x) (cg x)) (tree_ens (g x) (cg x)))
+  : (let c = TCbindP #a #b #wp #g pre post cg in
+     repr_steel_t (SH.KGhostI opened) b pre post (tree_req _ c) (tree_ens _ c))
+  = 
+    FStar.Monotonic.Pure.elim_pure_wp_monotonicity wp;
+    SH.ghostI_f (fun () ->
+    let x = f () in
+    SH.ghostI_u (rg x) ())
+
+inline_for_extraction noextract
+let bindP_ghost_steel0
+      (a : Type) (b : Type) (opened : Mem.inames) (wp : pure_wp a) ($f : unit -> PURE a wp) (g : (a -> prog_tree b))
+      (pre : pre_t) (post : post_t b)
+      (cg : ((x : a) -> tree_cond (g x) pre post))
+      (rg : (x : a) -> repr_steel_t (SH.KGhost opened) b pre post (tree_req (g x) (cg x)) (tree_ens (g x) (cg x)))
   : (let c = TCbindP #a #b #wp #g pre post cg in
      repr_steel_t (SH.KGhost opened) b pre post (tree_req _ c) (tree_ens _ c))
   =
@@ -337,18 +462,44 @@ let bindP_ghost_steel
     let x = f () in
     SH.ghost_u (rg x) ())
 
+inline_for_extraction noextract
+let bindP_ghost_steel
+      (a : Type) (b : Type) (opened : Mem.inames) (wp : pure_wp a) ($f : unit -> GHOST a wp) (g : (a -> prog_tree b))
+      (pre : pre_t) (post : post_t b)
+      (cg : ((x : a) -> tree_cond (g x) pre post))
+      (rg : (x : a) -> repr_steel_t (SH.KGhost opened) b pre post (tree_req (g x) (cg x)) (tree_ens (g x) (cg x)))
+  : (let c = TCbindP #a #b #wp #g pre post cg in
+     repr_steel_t (SH.KGhost opened) b pre post (tree_req _ c) (tree_ens _ c))
+  =
+    FStar.Monotonic.Pure.elim_pure_wp_monotonicity wp;
+    SH.ghost_f #opened (fun () ->
+    let x = f () in
+    SH.ghost_u (rg x) ())
+
+#push-options "--ifuel 1 --fuel 1 --z3rlimit 10"
 [@@ __repr_M__]
 inline_for_extraction noextract
-let bindP (#a #b : Type) (wp : pure_wp a) ($f : unit -> PURE a wp) (g : a -> repr SH.KSteel b)
-  : repr SH.KSteel b
+let bindP_ek (#a #b : Type) (ek : SH.effect_kind) (wp : pure_wp a) ($f : unit -> PURE a wp) (g : a -> repr ek b)
+  : repr ek b
   = {
     repr_tree  = TbindP a b wp (fun x -> (g x).repr_tree);
     repr_steel = (fun pre0 post0 c ->
                     let (TCbindP #a' #b' #wp #tg pre post cg) = c in
-                    let rg (x : a) : repr_steel_t SH.KSteel b pre post _ _
+                    let rg (x : a) : repr_steel_t ek b pre post _ _
                                    = (g x).repr_steel _ _ (cg x) in
-                    bindP_steel a b wp f tg pre post cg rg)
+                    match ek returns repr_steel_t ek b _ _ _ _ with
+                    | SH.KSteel    -> bindP_steel        a b   wp f tg pre post cg rg
+                    | SH.KAtomic o -> bindP_atomic_steel a b o wp f tg pre post cg rg
+                    | SH.KGhostI o -> bindP_ghostI_steel a b o wp f tg pre post cg rg
+                    | SH.KGhost  o -> bindP_ghost_steel0 a b o wp f tg pre post cg rg
+                 )
   }
+
+[@@ __repr_M__]
+inline_for_extraction noextract
+let bindP (#a #b : Type) (wp : pure_wp a) ($f : unit -> PURE a wp) (g : a -> repr SH.KSteel b)
+  : repr SH.KSteel b
+  = bindP_ek SH.KSteel wp f g
 
 [@@ __repr_M__]
 inline_for_extraction noextract
@@ -378,28 +529,6 @@ let ite_steel
      repr_steel_t SH.KSteel a pre post (tree_req _ c) (tree_ens _ c))
   = SH.steel_f (fun () ->
     if guard then SH.steel_u rthn () else SH.steel_u rels ())
-
-// Versions with the guard value as an hypothesis, used to define the if_then_else of an effect
-inline_for_extraction noextract
-let ite_steel_thn
-      (a : Type) (guard : bool) (thn : prog_tree a) (els : prog_tree a)
-      (pre : pre_t) (post : post_t a) (cthn : tree_cond thn pre post) (cels : tree_cond els pre post)
-      ($rthn : repr_steel_t SH.KSteel a pre post (tree_req thn cthn) (tree_ens thn cthn))
-      (_ : squash guard)
-  : (let c = TCif #a #guard #thn #els pre post cthn cels in
-     repr_steel_t SH.KSteel a pre post (tree_req _ c) (tree_ens _ c))
-  = SH.steel_f (fun () -> SH.steel_u rthn ())
-
-inline_for_extraction noextract
-let ite_steel_els
-      (a : Type) (guard : bool) (thn : prog_tree a) (els : prog_tree a)
-      (pre : pre_t) (post : post_t a) (cthn : tree_cond thn pre post) (cels : tree_cond els pre post)
-      ($rels : repr_steel_t SH.KSteel a pre post (tree_req els cels) (tree_ens els cels))
-      (_ : squash (~guard))
-  : (let c = TCif #a #guard #thn #els pre post cthn cels in
-     repr_steel_t SH.KSteel a pre post (tree_req _ c) (tree_ens _ c))
-  = SH.steel_f (fun () -> SH.steel_u rels ())
-
 
 inline_for_extraction noextract
 let ite_ghost_steel
@@ -439,7 +568,153 @@ let ite_ghost (#a : Type) (#opened : Mem.inames) (guard : bool) (thn els : repr 
   }
 
 
-(****** SteelGhost to Steel *)
+
+(*** Lifts *)
+
+(***** [erasable_t] *)
+
+type revealed_value (#a : Type) (x : Ghost.erased a) =
+  x' : a { x' == Ghost.reveal x }
+
+noeq inline_for_extraction noextract
+type erasable_t (a : Type) = {
+  erasable_rv : (x : Ghost.erased a) -> revealed_value x
+}
+
+private
+let __build_revealed_value (a : Type) : (x : Ghost.erased a) -> GTot (revealed_value x)
+  = fun x -> Ghost.reveal x
+
+// TODO: exceptions
+/// Solves a goal [erasable_t a] if a is an erasable type.
+let build_erasable_t () : T.Tac unit
+  = T.(
+    let a : term
+      = match inspect (cur_goal ()) with
+        | Tv_App  _ arg -> arg._1
+        | _ -> fail "build_erasable_t : goal"
+    in
+    apply (`Mkerasable_t);
+    // The following requires a conversion from [_ -> GTot (revealed_value x)] to [_ -> Tot (revealed_value x)]
+    // which succeeds iff [revealed_value x] (i.e. [a]) is erasable.
+    // Since we use (`#a), this may generate some guards to retypecheck (`#a).
+    with_policy SMT (fun () ->
+    exact (`(__build_revealed_value (`#a) <: _ -> Tot _)))
+  )
+
+private
+let test_erasable_unit : erasable_t unit
+  = _ by (build_erasable_t ())
+
+private
+let test_erasable_unit' : erasable_t U.unit'
+  = _ by (build_erasable_t ())
+
+#push-options "--silent"
+[@@ expect_failure [228]]
+private
+let test_erasable_int : erasable_t int
+  = _ by (build_erasable_t ())
+#pop-options
+
+[@@ erasable]
+private noeq
+type test_guard_type (_ : squash (forall (n : nat) . n >= 0)) =
+
+private
+let test_erasable_guard : erasable_t (test_guard_type ())
+  = _ by (build_erasable_t ())
+
+
+(***** [steel_liftable] *)
+
+// named as in Coq
+noeq
+type clos_refl_trans_1n (#a : Type) (r : a -> a -> Type) (x : a) : a -> Type =
+  | Rt1n_refl  : clos_refl_trans_1n r x x
+  | Rt1n_trans : (y : a) -> (z : a) ->
+                 r x y -> clos_refl_trans_1n r y z -> clos_refl_trans_1n r x z
+
+noeq
+type steel_liftable1 (a : Type) : SH.effect_kind -> SH.effect_kind -> Type =
+  | Lift_ghost_ghostI  : erasable_t a -> (opened : Mem.inames) ->
+                         steel_liftable1 a (SH.KGhost     opened) (SH.KGhostI opened)
+  | Lift_ghostI_atomic : (opened : Mem.inames) ->
+                         steel_liftable1 a (SH.KGhostI    opened) (SH.KAtomic opened)
+  | Lift_atomic_steel  : steel_liftable1 a (SH.KAtomic Set.empty)  SH.KSteel
+
+type steel_liftable (a : Type) : SH.effect_kind -> SH.effect_kind -> Type
+  = clos_refl_trans_1n (steel_liftable1 a)
+
+
+/// We define the lift on [repr_steel_t] rather than on [SH.steel] because the latter option does not work
+/// with steel's tactic because of the abstract specifications.
+
+let repr_steel_lift_ghost_ghostI_aux
+      #a #pre #post #req #ens #opened (f : repr_steel_t (SH.KGhost opened) a pre post req ens)
+  : SH.unit_steel_ghost (Ghost.erased a) opened
+      (vprop_of_list pre) (fun x -> vprop_of_list (post (Ghost.reveal x)))
+      (fun h0 -> req (sel_f pre h0))
+      (fun h0 x h1 -> ens (sel_f pre h0) (Ghost.reveal x) (sel_f (post (Ghost.reveal x)) h1))
+  =
+    fun () ->
+      let x = SH.ghost_u f () in
+      Ghost.hide x
+
+inline_for_extraction noextract
+let repr_steel_lift_ghost_ghostI
+      #a #pre #post #req #ens opened (e : erasable_t a) (f : repr_steel_t (SH.KGhost opened) a pre post req ens)
+  : repr_steel_t (SH.KGhostI opened) a pre post req ens
+  =
+    SH.ghostI_f (fun () ->
+      let x : Ghost.erased a = repr_steel_lift_ghost_ghostI_aux f () in
+      let x' : a = e.erasable_rv x in
+      change_equal_slprop (vprop_of_list (post (Ghost.reveal x))) (vprop_of_list (post x'));
+      Steel.Effect.Atomic.return x'
+  )
+
+inline_for_extraction noextract
+let repr_steel_lift_ghostI_atomic
+      #a #pre #post #req #ens opened (f : repr_steel_t (SH.KGhostI opened) a pre post req ens)
+  : repr_steel_t (SH.KAtomic opened) a pre post req ens
+  = SH.atomic_f (fun () -> SH.ghostI_u f ())
+
+inline_for_extraction noextract
+let repr_steel_lift_atomic_steel
+      #a #pre #post #req #ens (f : repr_steel_t (SH.KAtomic Set.empty) a pre post req ens)
+  : repr_steel_t SH.KSteel a pre post req ens
+  = SH.steel_f (fun () -> SH.atomic_u f ())
+
+inline_for_extraction noextract
+let repr_steel_lift1
+      (#a : Type) (#pre : pre_t) (#post : post_t a) (#req : req_t pre) (#ens : ens_t pre a post)
+      (#ek0 #ek1 : SH.effect_kind) (l : steel_liftable1 a ek0 ek1)
+      (f : repr_steel_t ek0 a pre post req ens)
+  : repr_steel_t ek1 a pre post req ens
+  = match l with
+  | Lift_ghost_ghostI e o -> repr_steel_lift_ghost_ghostI  o e f
+  | Lift_ghostI_atomic  o -> repr_steel_lift_ghostI_atomic o   f
+  | Lift_atomic_steel     -> repr_steel_lift_atomic_steel      f
+
+inline_for_extraction noextract
+let rec repr_steel_lift
+      (#a : Type) (#pre : pre_t) (#post : post_t a) (#req : req_t pre) (#ens : ens_t pre a post)
+      (#ek0 #ek1 : SH.effect_kind) (l : steel_liftable a ek0 ek1)
+      (f : repr_steel_t ek0 a pre post req ens)
+  : Tot (repr_steel_t ek1 a pre post req ens) (decreases l)
+  = match l with
+  | Rt1n_refl -> f
+  | Rt1n_trans _ _ l0 l1 -> repr_steel_lift l1 (repr_steel_lift1 l0 f)
+
+[@@ __repr_M__]
+inline_for_extraction noextract
+let repr_lift
+      (#a : Type) (#ek0 #ek1 : SH.effect_kind) (l : steel_liftable a ek0 ek1) (r : repr ek0 a)
+  : repr ek1 a
+  = { r with repr_steel = (fun pre post c -> repr_steel_lift l (r.repr_steel pre post c)) }
+
+
+(****** SteelGhost to Steel (Monad) *)
 
 inline_for_extraction noextract
 let ghost_to_steel_steel (a : Type) (t : prog_tree (Ghost.erased a)) (pre : pre_t) (post : post_t (Ghost.erased a))
@@ -458,39 +733,11 @@ let ghost_to_steel (#a : Type) (f : repr (SH.KGhost Set.empty) (Ghost.erased a))
                     ghost_to_steel_steel a f.repr_tree pre post c (f.repr_steel _ _ c))
   }
 
-
-inline_for_extraction noextract
-let ghost_to_steel_steel_ct_aux (a : Type) (t : prog_tree a) (pre : pre_t) (post : post_t a)
-      (c : tree_cond t pre post)
-      ($r : repr_steel_t (SH.KGhost Set.empty) a pre post (tree_req t c) (tree_ens t c))
-  : SteelGhost (Ghost.erased a) Set.empty
-             (vprop_of_list pre) (fun x -> vprop_of_list (post (Ghost.reveal x)))
-             (fun h0 -> tree_req t c (sel_f pre h0))
-             (fun h0 x h1 -> tree_ens t c (sel_f pre h0) (Ghost.reveal x) (sel_f (post (Ghost.reveal x)) h1))
-  = let x = SH.ghost_u r () in Ghost.hide x
-
-inline_for_extraction noextract
-let ghost_to_steel_steel_ct (a : Type) (t : prog_tree a) (pre : pre_t) (post : post_t a)
-      (c : tree_cond t pre post)
-      ($r : repr_steel_t (SH.KGhost Set.empty) a pre post (tree_req t c) (tree_ens t c))
-      (rv : (x : Ghost.erased a) -> (x' : a { x' == Ghost.reveal x }))
-  : repr_steel_t SH.KSteel a pre post (tree_req t c) (tree_ens t c)
-  = SH.steel_f (fun () ->
-    let x : Ghost.erased a = ghost_to_steel_steel_ct_aux a t pre post c r in
-    let x' : a = rv x in
-    change_equal_slprop (vprop_of_list (post (Ghost.reveal x))) (vprop_of_list (post x'));
-    Steel.Effect.Atomic.return x'
-  )
-
 [@@ __repr_M__]
 inline_for_extraction noextract
 let ghost_to_steel_ct (#a : Type) (f : repr (SH.KGhost Set.empty) a)
       (rv : (x : Ghost.erased a) -> (x' : a { x' == Ghost.reveal x }))
   : repr SH.KSteel a
-  = {
-    repr_tree  = f.repr_tree;
-    repr_steel = (fun pre post c ->
-                    ghost_to_steel_steel_ct a f.repr_tree pre post c (f.repr_steel _ _ c) rv)
-  }
-
-// TODO: SteelAtomic
+  = repr_lift (Rt1n_trans _ _ (Lift_ghost_ghostI ({erasable_rv = rv}) _)
+              (Rt1n_trans _ _ (Lift_ghostI_atomic _)
+              (Rt1n_trans _ _ Lift_atomic_steel Rt1n_refl))) f
