experiment/Experiment.Steel.Effect.Test.fst
@@ -1,5 +1,8 @@
 module Experiment.Steel.Effect.Test
 
+module SH  = Experiment.Steel.Steel
+module Mem = Steel.Memory
+
 open FStar.Tactics
 open Steel.Effect.Common
 open Steel.Reference
@@ -10,33 +13,36 @@ let display_term (#a : Type) (x : a) : Type = unit
 
 /// This retypecheck [r]. It fails if r contains a bind_pure since it will need to prove the monotonicity of the
 /// weakest precondition ([pure_wp_monotonic]).
-let dump_repr (#a : Type) (#r : prog_tree a)
-      ($re : unit -> MRepr a r)
+let dump_repr (#a : Type) (#r : prog_tree a) (ek : SH.effect_kind)
+      ($re : unit -> MRepr a ek r)
       (#[(norm [delta_attr [`%__repr_M__]; iota]; dump "dump_repr"; exact (`()))] d : display_term r)
       ()
   : unit
   = ()
 
 
+// We need to annotate [SH.KGhostI Set.empty] otherwise the infered effect is [SH.KGhostI ?opened] and
+// ?opened is not constrained
 let test0 =
-  dump_repr (fun () -> let x = return 5 in return (x + 1)) ()
+  dump_repr (SH.KGhostI Set.empty) (fun () -> let x = return 5 in return (x + 1)) ()
 
-//[@@ handle_smt_goals ] let tac () = Tactics.dump "SMT query"
-[@@ expect_failure [19]]
-let test1 = dump_repr (fun () -> assert (5 >= 0); return 5) ()
+#push-options "--no_smt"
+[@@ expect_failure [298]]
+let test1 = dump_repr (SH.KGhostI Set.empty) (fun () -> assert (5 >= 0); return 5) ()
+#pop-options
 
 let test1' (x : int)
   : usteel int emp (fun _ -> emp) (requires fun _ -> x >= 1) (ensures fun _ y _ -> y >= 5)
-  = to_steel #[Dump Stage_WP] begin fun () ->
+  = to_steel begin fun () ->
     assert (x >= 0);
     return (5 + x)
   end
-  
 
-//let test2 (r : ref int) =
-//  dump_repr (fun () -> let x = call read r in return x) ()
 
 // Stack overflow
+//let test2 (r : ref int) =
+//  dump_repr SH.KSteel (fun () -> let x = call read r in return x) ()
+
 //let test3 (b : bool) (r0 r1 : ref int) =
 //  dump_repr (fun () -> if b then let x = read r0 in return x
 //                         else let x = read r1 in return x)
@@ -45,7 +51,7 @@ let test3' (b : bool) (r0 r1 : ref int)
   : usteel int (vptr r0 `star` vptr r1) (fun _ -> vptr r0 `star` vptr r1)
          (requires fun h0 -> sel r0 h0 >= 0 /\ sel r1 h0 >= 0)
          (ensures  fun h0 x h1 -> frame_equalities (vptr r0 `star` vptr r1) h0 h1 /\ x >= 0)
-  = to_steel #[Timer] begin fun () ->
+  = to_steel begin fun () ->
     if b then call read r0 else call read r1
   end
 
@@ -77,4 +83,32 @@ let test5' (r : ref nat)
   = to_steel begin fun () ->
     let x = call read r in
     call (write r) (x - 1)
+  end
+
+
+let test6 (opened : Mem.inames) (r : ghost_ref int) (x : int)
+  : usteel_ghost unit opened
+      (ghost_vptr r) (fun _ -> ghost_vptr r) (fun _ -> True) (fun _ _ _ -> True)
+  = to_steel_g begin fun () ->
+    call_g (ghost_write r) x;
+    call_g (ghost_write r) x
+  end
+
+// MRepr _ (SH.KGhost _) is not erasable and we cannot define a polymonadic bind with GHOST
+[@@ expect_failure]
+let test7 (opened: Mem.inames) (r : ghost_ref int)
+  : usteel_ghost int opened
+      (ghost_vptr r) (fun _ -> ghost_vptr r) (fun _ -> True) (fun _ _ _ -> True)
+  = to_steel_g begin fun () ->
+    let x = call_g ghost_read r in
+    return_g (Ghost.reveal x)
+  end
+
+let test8 (opened : Mem.inames) (r : ghost_ref int) (b : bool) (x0 x1 : int)
+  : usteel_ghost unit opened
+      (ghost_vptr r) (fun _ -> ghost_vptr r) (fun _ -> True) (fun _ _ _ -> True)
+  = to_steel_g begin fun () ->
+    if b
+    then call_g (ghost_write r) x0
+    else call_g (ghost_write r) x1
   end
