experiment/Experiment.Steel.Effect.fst
@@ -1,13 +1,15 @@
 module Experiment.Steel.Effect
 
-module U  = Learn.Util
-module M  = Experiment.Steel.Repr.M
-module C  = Experiment.Steel.Combinators
-module T  = FStar.Tactics
-module L  = FStar.List.Pure
-module UV = Learn.Universe
-module SE = Steel.Effect
-module SH = Experiment.Steel.Steel
+module U   = Learn.Util
+module M   = Experiment.Steel.Repr.M
+module C   = Experiment.Steel.Combinators
+module T   = FStar.Tactics
+module L   = FStar.List.Pure
+module UV  = Learn.Universe
+module SE  = Steel.Effect
+module SA  = Steel.Effect.Atomic
+module SH  = Experiment.Steel.Steel
+module Mem = Steel.Memory
 
 open Experiment.Steel.Interface
 
@@ -16,7 +18,7 @@ open Experiment.Steel.Interface
 irreducible let __mrepr_implicit__ : unit = ()
 
 
-(**** MRepr effect *)
+(*** MRepr effect *)
 
 /// We fix the universe [u#p] of the types in bind_pure to [u#8].
 /// Values in lower universes are raised.
@@ -26,16 +28,32 @@ irreducible let __mrepr_implicit__ : unit = ()
 unfold
 type prog_tree = M.prog_tree u#a u#8
 
-type repr' (a : Type) (t : M.prog_tree u#a u#p a) : Type
-  = r : M.repr u#a u#p SH.KSteel a { r.repr_tree == t }
+type repr' (a : Type) (ek : SH.effect_kind) (t : M.prog_tree u#a u#p a) : Type
+  = r : M.repr u#a u#p ek a { r.repr_tree == t }
 
-type repr (a : Type) (t : prog_tree u#a a) : Type
-  = r : M.repr u#a u#8 SH.KSteel a { r.repr_tree == t }
+type repr (a : Type) (ek : SH.effect_kind) (t : prog_tree u#a a) : Type
+  = r : M.repr u#a u#8 ek a { r.repr_tree == t }
 
+
+(***** return *)
+
+let return_ghostI
+      (a : Type) (x : a) (#opened: Mem.inames)
+  : repr u#a a (SH.KGhostI opened) (M.Tret a x (fun _ -> []))
+  = C.return_ghostI_hint #a x (fun _ -> [])
+
+let return_ghost
+      (a : Type) (x : a) (#opened: Mem.inames)
+  : repr u#a a (SH.KGhost opened) (M.Tret a x (fun _ -> []))
+  = C.return_ghost #a x
+
+// FIXME
+//   if we replace SH.KGhostI by SH.KGhost, [test3'] fails because of some bind
+//   maybe we can infer when one should use return_ghostI/return_ghost
 let return_
-      (a : Type) (x : a)
-  : repr u#a a (M.Tret a x (fun _ -> []))
-  = C.return #a x
+      (a : Type) (x : a) (#[@@@ __mrepr_implicit__] opened: Mem.inames)
+  : repr u#a a (SH.KGhostI opened) (M.Tret a x (fun _ -> []))
+  = return_ghostI a x #opened
 
 (***** bind *)
 
@@ -43,26 +61,44 @@ let return_
 noeq inline_for_extraction
 type combine_bind_t
        (a : Type u#a) (b : Type u#b)
+       (ek0 ek1 ek : SH.effect_kind)
        (f : prog_tree a) (g : a -> prog_tree b)
 = {
   cb_bind_repr : prog_tree b;
-  cb_bind_impl : (rf : repr a f) -> (rg : ((x : a) -> repr b (g x))) ->
-                 repr b cb_bind_repr
+  cb_bind_impl : (rf : repr a ek0 f) -> (rg : ((x : a) -> repr b ek1 (g x))) ->
+                 repr b ek cb_bind_repr
+}
+
+type combinable_bind_repr (a0 a1 : Type u#a) (ek0 ek1 ek2 : SH.effect_kind)
+  = (f : M.repr u#a u#8 ek0 a0) -> (g : ((x : a0) -> M.repr u#a u#8 ek1 a1)) ->
+    repr a1 ek2 (M.Tbind a0 a1 f.repr_tree (fun x -> (g x).repr_tree))
+
+noeq inline_for_extraction
+type combinable_bind_t (a0 a1 : Type u#a) (ek0 ek1 ek2 : SH.effect_kind) = {
+  cba_bind_ek0'  : SH.effect_kind;
+  cba_bind_ek1'  : SH.effect_kind;
+  cba_bind_repr  : combinable_bind_repr a0 a1 cba_bind_ek0' cba_bind_ek1' ek2;
+  cba_bind_lift0 : C.steel_liftable a0 ek0 cba_bind_ek0';
+  cba_bind_lift1 : C.steel_liftable a1 ek1 cba_bind_ek1';
 }
 
 [@@ __repr_M__]
 inline_for_extraction
 let combine_bind
-      (a : Type u#b) (b : Type u#b) 
+      (a : Type u#b) (b : Type u#b)
+      (ek0 ek1 ek2 : SH.effect_kind)
+      (cba : combinable_bind_t a b ek0 ek1 ek2)
       (f : prog_tree a) (g : a -> prog_tree b)
-  : combine_bind_t a b f g
+  : combine_bind_t a b ek0 ek1 ek2 f g
   = {
     cb_bind_repr = M.Tbind a b f (fun x -> g x); // We need the functional extensionality so we eta-expend g
     cb_bind_impl = (fun rf rg ->
-                      U.funext_eta (fun x -> g x) (fun x -> (rg x).repr_tree)
+                      let rf' = C.repr_lift cba.cba_bind_lift0 rf             in
+                      let rg' (x : a) = C.repr_lift cba.cba_bind_lift1 (rg x) in
+                      U.funext_eta (fun x -> g x) (fun x -> (rg' x).repr_tree)
                         (U.by_refl ()) (U.by_refl ())
                         (fun x -> ());
-                      C.bind #a #b rf rg);
+                      cba.cba_bind_repr rf' rg');
   }
 
 /// Since we want to represent the program as a tree, we need [u#a == u#b]. However when defining an effect,
@@ -73,82 +109,128 @@ let combine_bind
 /// The tactic will fail if [u#a <> u#b].
 let bind_
       (a : Type u#a) (b : Type u#b)
+      (#ek0 #ek1 #ek : SH.effect_kind)
       (#f : prog_tree a) (#g : a -> prog_tree b)
       (#[@@@ __mrepr_implicit__] cb
-        : (f : prog_tree a) -> (g : (a -> prog_tree b)) -> combine_bind_t a b f g)
-      (rf : repr u#a a f) (rg : (x : a) -> repr u#b b (g x))
-  : repr u#b b (cb f g).cb_bind_repr
+        : (f : prog_tree a) -> (g : (a -> prog_tree b)) -> combine_bind_t a b ek0 ek1 ek f g)
+      (rf : repr u#a a ek0 f) (rg : (x : a) -> repr u#b b ek1 (g x))
+  : repr u#b b ek (cb f g).cb_bind_repr
   = (cb f g).cb_bind_impl rf rg
 
 
 (***** subcomp *)
 
 type combine_subcomp_t
-      (a : Type u#a) (f : prog_tree a) (g : prog_tree a)
-  = repr a f -> repr a g
+      (a : Type u#a) (ek0 ek1 : SH.effect_kind) (f : prog_tree a) (g : prog_tree a)
+  = repr a ek0 f -> repr a ek1 g
 
+// TODO?: allow lifting effect_kind
 let combine_subcomp_refl
-      (a : Type u#a) (f : prog_tree a)
-  : combine_subcomp_t a f f
+      (a : Type u#a) (ek : SH.effect_kind) (f : prog_tree a)
+  : combine_subcomp_t a ek ek f f
   = fun rf -> rf
 
 let subcomp
       (a : Type u#a)
+      (#ek0 : SH.effect_kind) (#ek1 : SH.effect_kind)
       (#f : prog_tree a) (#g : prog_tree a)
-      (#[@@@ __mrepr_implicit__] cb : combine_subcomp_t a f g)
-      (rf : repr a f)
-  : repr a g
+      (#[@@@ __mrepr_implicit__] cb : combine_subcomp_t a ek0 ek1 f g)
+      (rf : repr a ek0 f)
+  : repr a ek1 g
   = cb rf
 
 
 (***** if then else *)
 
+noeq
+type combinable_ite_t (a : Type) (ek0 ek1 ek2 : SH.effect_kind) = {
+  cba_ite_restr : squash (~ (SH.KAtomic? ek2)); // We match the restriction of SteelAtomic, but we do not need it
+  cba_ite_lift0 : C.steel_liftable a ek0 ek2;
+  cba_ite_lift1 : C.steel_liftable a ek1 ek2;
+}
+
 let if_then_else
       (a : Type)
+      (#ek0 #ek1 #ek2 : SH.effect_kind)
       (#thn : prog_tree a) (#els : prog_tree a)
-      (rthn : repr a thn) (rels : repr a els)
+      (#[@@@ __mrepr_implicit__] cb : combinable_ite_t a ek0 ek1 ek2)
+      (rthn : repr a ek0 thn) (rels : repr a ek1 els)
       (guard : bool)
   : Type
-  = repr a (M.Tif a guard thn els)
+  = repr a ek2 (M.Tif a guard thn els)
+
+
+inline_for_extraction noextract
+let ite_steel_thn
+      (a : Type) (ek : SH.effect_kind) (guard : bool) (thn : M.prog_tree a) (els : M.prog_tree a)
+      (pre : M.pre_t) (post : M.post_t a) (cthn : M.tree_cond thn pre post) (cels : M.tree_cond els pre post)
+      ($rthn : M.repr_steel_t ek a pre post (M.tree_req thn cthn) (M.tree_ens thn cthn))
+      (_ : squash guard)
+  : (let c = M.TCif #a #guard #thn #els pre post cthn cels in
+     M.repr_steel_t ek a pre post (M.tree_req _ c) (M.tree_ens _ c))
+  = M.repr_steel_subcomp ek _ _ _ _ (fun _ -> ()) (fun _ _ _ -> ()) rthn
+
+inline_for_extraction noextract
+let ite_steel_els
+      (a : Type) (ek : SH.effect_kind) (guard : bool) (thn : M.prog_tree a) (els : M.prog_tree a)
+      (pre : M.pre_t) (post : M.post_t a) (cthn : M.tree_cond thn pre post) (cels : M.tree_cond els pre post)
+      ($rels : M.repr_steel_t ek a pre post (M.tree_req els cels) (M.tree_ens els cels))
+      (_ : squash (~ guard))
+  : (let c = M.TCif #a #guard #thn #els pre post cthn cels in
+     M.repr_steel_t ek a pre post (M.tree_req _ c) (M.tree_ens _ c))
+  = M.repr_steel_subcomp ek _ _ _ _ (fun _ -> ()) (fun _ _ _ -> ()) rels
+
 
 let ite_combine_thn
-      (a : Type) (guard : bool) (thn els : prog_tree a)
+      (a : Type) (ek0 ek1 : SH.effect_kind) (guard : bool) (thn els : prog_tree a)
       (_ : squash guard)
-  : combine_subcomp_t a thn (M.Tif a guard thn els)
+      (l : C.steel_liftable a ek0 ek1)
+  : combine_subcomp_t a ek0 ek1 thn (M.Tif a guard thn els)
   = fun rthn -> {
     repr_tree  = M.Tif a guard thn els;
     repr_steel = (fun pre0 post0 c ->
                     let M.TCif pre post cthn cels = c in
-                    C.ite_steel_thn a guard thn els pre post cthn cels (rthn.repr_steel _ _ cthn) ())
+                    ite_steel_thn a ek1 guard thn els pre post cthn cels
+                         ((C.repr_lift l rthn).repr_steel _ _  cthn) ())
   }
 
 let ite_combine_els
-      (a : Type) (guard : bool) (thn els : prog_tree a)
+      (a : Type) (ek0 ek1 : SH.effect_kind) (guard : bool) (thn els : prog_tree a)
       (_ : squash (~guard))
-  : combine_subcomp_t a els (M.Tif a guard thn els)
+      (l : C.steel_liftable a ek0 ek1)
+  : combine_subcomp_t a ek0 ek1 els (M.Tif a guard thn els)
   = fun rels -> {
     repr_tree  = M.Tif a guard thn els;
     repr_steel = (fun pre0 post0 c ->
                     let M.TCif pre post cthn cels = c in
-                    C.ite_steel_els a guard thn els pre post cthn cels (rels.repr_steel _ _ cels) ())
+                    ite_steel_els a ek1 guard thn els pre post cthn cels
+                          ((C.repr_lift l rels).repr_steel _ _ cels) ())
   }
 
 
-irreducible let __ite_soundness__ : unit = ()
+private irreducible
+let __ite_soundness__ : unit = ()
 
 [@@ resolve_implicits; __ite_soundness__]
 let ite_soundness_tac () : T.Tac unit
   = T.(
+    let exact_hyp () =
+      first (map (fun (b : binder) () -> exact b <: Tac unit) (cur_binders ()))
+    in
     iterAll (fun () -> try trefl () with _ -> ());
     norm [delta_only [`%pure_null_wp0]; simplify]; trivial ();
     first [(fun () -> apply (`ite_combine_thn)); (fun () -> apply (`ite_combine_els))];
-    smt ()
+    smt ();
+    first [
+      (fun () -> apply (`Mkcombinable_ite_t?.cba_ite_lift0); exact_hyp ());
+      (fun () -> apply (`Mkcombinable_ite_t?.cba_ite_lift1); exact_hyp ())
+    ]
   )
 
 
 [@@ ite_soundness_by __ite_soundness__]
 total reflectable effect {
-  MRepr (a : Type) (r : prog_tree a)
+  MRepr (a : Type) (ek : SH.effect_kind) (r : prog_tree a)
   with {
     repr;
     return = return_;
@@ -158,9 +240,13 @@ total reflectable effect {
   }
 }
 
-let return (#a : Type u#a) (x : a)
-  : MRepr a (M.Tret a x (fun _ -> []))
-  = MRepr?.reflect (return_ a x)
+let return (#a : Type u#a) (#opened : Mem.inames) (x : a)
+  : MRepr a (SH.KGhostI opened) (M.Tret a x (fun _ -> []))
+  = MRepr?.reflect (return_ghostI a x #opened)
+
+let return_g (#a : Type u#a) (#opened : Mem.inames) (x : a)
+  : MRepr a (SH.KGhost opened) (M.Tret a x (fun _ -> []))
+  = MRepr?.reflect (return_ghost a x #opened)
 
 
 (***** bind (PURE, MRepr) |> MRepr *)
@@ -169,11 +255,12 @@ let return (#a : Type u#a) (x : a)
 noeq inline_for_extraction
 type combine_bind_pure_t
        (a : Type u#r) (b : Type u#a)
+       (ek : SH.effect_kind)
        (wp : pure_wp a) (g : a -> M.prog_tree u#a u#p b)
 = {
   cb_bindP_repr : M.prog_tree u#a u#p b;
-  cb_bindP_impl : (rf : unit -> PURE a wp) -> (rg : ((x : a) -> repr' b (g x))) ->
-                  repr' u#a u#p b cb_bindP_repr
+  cb_bindP_impl : (rf : unit -> PURE a wp) -> (rg : ((x : a) -> repr' b ek (g x))) ->
+                  repr' u#a u#p b ek cb_bindP_repr
 }
 
 /// This should be applied with [u#r <= u#8] so [u#(max r 8) = u#8]
@@ -181,9 +268,10 @@ type combine_bind_pure_t
 inline_for_extraction
 let combine_bind_pure
       (a : Type u#r) (b : Type u#a)
+      (ek : SH.effect_kind)
       (wp : pure_wp a) (g : a -> M.prog_tree u#a u#(max r 8) b)
       
-  : combine_bind_pure_t u#r u#a u#(max r 8) a b wp g
+  : combine_bind_pure_t u#r u#a u#(max r 8) a b ek wp g
   = 
     let t = M.TbindP (UV.raise_t u#r u#8 a) b
                      (UV.raise_pure_wp u#r u#8 wp) (UV.lift_dom g) in
@@ -191,28 +279,29 @@ let combine_bind_pure
     cb_bindP_repr = t;
     cb_bindP_impl = (fun rf rg ->
                        let rg' = UV.lift_dom rg in
-                       let r = C.bindP #(UV.raise_t u#r u#8 a) #b (UV.raise_pure_wp u#r u#8 wp)
-                                       (UV.raise_pure_val wp rf) rg'
+                       let r = C.bindP_ek #(UV.raise_t u#r u#8 a) #b ek (UV.raise_pure_wp u#r u#8 wp)
+                                          (UV.raise_pure_val wp rf) rg'
                        in
                        U.funext_eta (UV.lift_dom g) (fun x -> (rg' x).repr_tree)
                          (U.by_refl ()) (U.by_refl ())
                          (fun x -> ());
                        assert (r.repr_tree == t)
                          by T.(norm [delta_only [`%M.Mkrepr?.repr_tree]];
-                               norm [delta_only [`%C.bindP]; iota];
+                               norm [delta_only [`%C.bindP_ek]; iota];
                                smt ());
                        r)
   }
 
 let bind_pure_mrepr
       (a : Type u#r) (b : Type u#a)
+      (#ek : SH.effect_kind)
       (#wp : pure_wp a)
       (#g : a -> prog_tree b)
       (#[@@@ __mrepr_implicit__] cb
-        : (wp : pure_wp a) -> (g : (a -> prog_tree b)) -> combine_bind_pure_t u#r u#a u#8 a b wp g)
+        : (wp : pure_wp a) -> (g : (a -> prog_tree b)) -> combine_bind_pure_t u#r u#a u#8 a b ek wp g)
       (rf : eqtype_as_type unit -> PURE a wp)
-      (rg : (x : a) -> repr b (g x))
-  : repr b (cb wp g).cb_bindP_repr
+      (rg : (x : a) -> repr b ek (g x))
+  : repr b ek (cb wp g).cb_bindP_repr
   = (cb wp g).cb_bindP_impl rf rg
 
 #push-options "--warn_error -330"
@@ -220,7 +309,7 @@ polymonadic_bind (PURE, MRepr) |> MRepr = bind_pure_mrepr
 #pop-options
 
 
-(***** lifting Steel.Effect.SteelBase ~> MRepr *)
+(***** lifting Steel ~> MRepr *)
 
 /// The sub_effect is not working (order of resolution of the implicits, use of Steel's combinators instead of
 /// MRepr's combinators, Steel computation unexpectedly lifted where MRepr does not appear).
@@ -231,7 +320,7 @@ let lift_steel_mrepr
       (a : Type) (pre : SE.pre_t) (post : SE.post_t a)
       (req : SE.req_t pre) (ens : SE.ens_t pre a post)
       (f : Steel.Effect.repr a false pre post req ens)
-  : repr a M.(Tspec a (spec_r_steel u#a u#8 pre post req ens))
+  : repr a SH.KSteel M.(Tspec a (spec_r_steel u#a u#8 pre post req ens))
   = C.repr_of_steel #a pre post req ens
       (fun () -> SE.SteelBase?.reflect f)
   
@@ -243,20 +332,28 @@ let call (#b : Type u#b)
       (#a : b -> Type) (#pre : b -> SE.pre_t) (#post : (x : b) -> SE.post_t (a x))
       (#req : (x : b) -> SE.req_t (pre x)) (#ens : (x : b) -> SE.ens_t (pre x) (a x) (post x))
       ($f : (x : b) -> SE.Steel (a x) (pre x) (post x) (req x) (ens x)) (x : b)
-  : MRepr (a x) (M.Tspec (a x) (M.spec_r_steel u#a u#8 (pre x) (post x) (req x) (ens x)))
+  : MRepr (a x) SH.KSteel (M.Tspec (a x) (M.spec_r_steel u#a u#8 (pre x) (post x) (req x) (ens x)))
   = MRepr?.reflect (C.repr_of_steel #(a x) (pre x) (post x) (req x) (ens x) (fun () -> f x))
 
+unfold
+let call_g (#b : Type u#b)
+      (#a : b -> Type) (#opened : b -> Mem.inames) (#pre : b -> SE.pre_t) (#post : (x : b) -> SE.post_t (a x))
+      (#req : (x : b) -> SE.req_t (pre x)) (#ens : (x : b) -> SE.ens_t (pre x) (a x) (post x))
+      ($f : (x : b) -> SA.SteelGhost (a x) (opened x) (pre x) (post x) (req x) (ens x)) (x : b)
+  : MRepr (a x) (SH.KGhost (opened x)) (M.Tspec (a x) (M.spec_r_steel u#a u#8 (pre x) (post x) (req x) (ens x)))
+  = MRepr?.reflect (C.repr_of_steel_ghost #(a x) (pre x) (post x) (req x) (ens x) (fun () -> f x))
 
-(**** Conversion to Steel *)
+
+(*** Conversion to Steel *)
 
 /// [ConvEffect] is a dummy effect whose only purpose is to avoid the retypechecking of [prog_tree] that would
 /// happen if it appeared outside effect combinators.
 
-type cv_repr (a : Type u#a) (pre : SE.pre_t) (post : SE.post_t a)
+type cv_repr (a : Type u#a) (ek : SH.effect_kind) (pre : SE.pre_t) (post : SE.post_t a)
              (req : SE.req_t pre) (ens : SE.ens_t pre a post)
              (flags : list flag)
   : Type
-  = SH.unit_steel a pre post req ens
+  = SH.steel a pre post req ens ek
 
 /// [ConvEffect] is only used to convert a [MRepr] into a [SH.unit_steel]. Its combinators (return, bind,
 /// lifting of pure) should never be used.
@@ -273,7 +370,7 @@ noeq type cv_unused =
 let elim_cv_unused (#a : Type) (u : cv_unused) : a
   = match u with
 
-unfold let dummy_cv (a : Type u#a) = cv_repr a SE.emp (fun _ -> SE.emp) (fun _ -> True) (fun _ _ _ -> True) []
+unfold let dummy_cv (a : Type u#a) = cv_repr a SH.KSteel SE.emp (fun _ -> SE.emp) (fun _ -> True) (fun _ _ _ -> True) []
 
 let cv_return
       (a : Type u#a) (x : a) (#[@@@ __cv_unused__] u : cv_unused)
@@ -282,6 +379,7 @@ let cv_return
 
 let cv_bind
       (a : Type u#a) (b : Type u#b)
+      (#ek0 #ek1 : SH.effect_kind)
       (#pre_f : SE.pre_t) (#post_f : SE.post_t a)
       (#req_f : SE.req_t pre_f) (#ens_f : SE.ens_t pre_f a post_f)
       (#fsf : list flag)
@@ -289,8 +387,8 @@ let cv_bind
       (#req_g : (x : a) -> SE.req_t (pre_g x)) (#ens_g : (x : a) -> SE.ens_t (pre_g x) b (post_g x))
       (#fsg : (x : a) -> list flag)
       (#[@@@ __cv_unused__] u : cv_unused)
-      (f : cv_repr a pre_f post_f req_f ens_f fsf)
-      (g : (x : a) -> cv_repr b (pre_g x) (post_g x) (req_g x) (ens_g x) (fsg x))
+      (f : cv_repr a ek0 pre_f post_f req_f ens_f fsf)
+      (g : (x : a) -> cv_repr b ek1 (pre_g x) (post_g x) (req_g x) (ens_g x) (fsg x))
   : dummy_cv b
   = elim_cv_unused u
 
@@ -299,7 +397,7 @@ let cv_bind
 [@@ allow_informative_binders]
 total reifiable effect {
   ConvEffect
-    (a : Type) (pre : SE.pre_t) (post : SE.post_t a)
+    (a : Type) (ek : SH.effect_kind) (pre : SE.pre_t) (post : SE.post_t a)
     (req : SE.req_t pre) (ens : SE.ens_t pre a post)
     (flags : list flag)
   with {
@@ -320,27 +418,28 @@ let lift_pure_cv
 sub_effect PURE ~> ConvEffect = lift_pure_cv
 
 
-
 noeq
 type mrepr_to_steel_t
        (flags : list flag)
-       (a : Type) (pre : SE.pre_t) (post : SE.post_t a) (req : SE.req_t pre) (ens : SE.ens_t pre a post)
+       (a : Type) (ek : SH.effect_kind)
+       (pre : SE.pre_t) (post : SE.post_t a) (req : SE.req_t pre) (ens : SE.ens_t pre a post)
        (t : prog_tree a)
-  = | MReprToSteel of (repr a t -> SH.unit_steel a pre post req ens)
+  = | MReprToSteel of (repr a ek t -> SH.steel a pre post req ens ek)
 
 let lift_mrepr_cv
-      (a : Type) (t : prog_tree a)
+      (a : Type) (ek0 ek1 : SH.effect_kind) (t : prog_tree a)
       (pre : SE.pre_t) (post : SE.post_t a) (req : SE.req_t pre) (ens : SE.ens_t pre a post) (flags : list flag)
-      ([@@@ __mrepr_implicit__] cv : mrepr_to_steel_t flags a pre post req ens t)
-      (r : repr a t)
-  : cv_repr a pre post req ens flags
+      ([@@@ __mrepr_implicit__] lt : C.steel_liftable a ek0 ek1)
+      ([@@@ __mrepr_implicit__] cv : mrepr_to_steel_t flags a ek1 pre post req ens t)
+      (r : repr a ek0 t)
+  : cv_repr a ek1 pre post req ens flags
   = let MReprToSteel cv = cv in
-    cv r
+    cv (C.repr_lift lt r)
 
 sub_effect MRepr ~> ConvEffect = lift_mrepr_cv
 
 
-(**** Implicits resolution *)
+(*** Implicits resolution *)
 
 module ES   = Experiment.Steel
 module LV   = Experiment.Steel.Repr.LV
@@ -349,6 +448,226 @@ module TcS  = Experiment.Steel.Tac
 open FStar.Tactics
 open Learn.Tactics.Util
 
+// TODO: better errors
+
+private noeq
+type filter_goals_r = {
+  // combinable_bind_t, combinable_ite_t
+  fgoals_comb : list goal;
+  // steel_liftable
+  fgoals_lift : list goal;
+  // mrepr_to_steel_t
+  fgoals_tstl : list goal;
+}
+
+let rec mrepr_implicits_init (r : filter_goals_r) : Tac filter_goals_r
+  =
+    match goals () with
+    | [] -> r
+    | g :: _ ->
+      let r =
+        if not (Tv_Uvar? (goal_witness g))
+        then (dismiss (); r) // the goal has already been solved
+        else begin
+          let hd = try collect_fvar (collect_app (goal_type g))._1
+                   with _ -> fail "unexpected shape"
+          in
+          // The only sources of failure here should be a bind where the two types involved belong to
+          // different universes. Or a polymonadic bind with an universe greater than [u#8].
+          if hd = (`%combine_bind_t)
+          then begin
+            apply (`combine_bind);
+            // combinable_bind_t
+            let g = _cur_goal () in
+            dismiss ();
+            {r with fgoals_comb = g :: r.fgoals_comb}
+          end else if hd = (`%combine_subcomp_t)
+          then (apply (`combine_subcomp_refl); r)
+          else if hd = (`%combine_bind_pure_t)
+          then (apply (`combine_bind_pure); r)
+
+          else if hd = (`%combinable_ite_t)
+          then (dismiss (); {r with fgoals_comb = g :: r.fgoals_comb})
+          else if hd = (`%C.steel_liftable)
+          then (dismiss (); {r with fgoals_lift = g :: r.fgoals_lift})
+          else if hd = (`%mrepr_to_steel_t)
+          then (dismiss (); {r with fgoals_tstl = g :: r.fgoals_tstl})
+          else if hd = (`%Mem.inames)
+          then (dismiss (); r) // should be inferred as side effects of other goals
+          else fail "unexpected shape"
+        end
+      in
+      mrepr_implicits_init r
+
+
+/// Solves a goal [C.steel_liftable a ek0 ek1] where the heads of [ek0] and [ek1] are known.
+let rec build_steel_liftable () : Tac unit
+  =
+    try apply (`C.Rt1n_refl)
+    with _ ->
+      apply (`C.Rt1n_trans);
+      // lift1
+      begin
+        match catch (fun () -> apply (`C.Lift_ghost_ghostI)) with
+        | Inr () -> C.build_erasable_t ()
+        | Inl _ ->
+        try apply (`C.Lift_ghostI_atomic) with _ ->
+        try apply (`C.Lift_atomic_steel)  with _ ->
+        fail "build_steel_liftable"
+      end;
+
+      build_steel_liftable ()
+  
+
+private
+type effect_kind_enum = | ESteel | EAtomic | EGhostI | EGhost
+
+private
+let ek_ord (ek : effect_kind_enum) : int
+  = match ek with
+  | EGhost  -> 0
+  | EGhostI -> 1
+  | EAtomic -> 2
+  | ESteel  -> 3
+
+private
+let ek_le (ek0 ek1 : effect_kind_enum) : bool
+  = ek_ord ek0 <= ek_ord ek1
+
+let collect_effect_kind (t : term) : Tac (option effect_kind_enum)
+  =
+    if Tv_Uvar? (inspect t) then None
+    else begin
+      let hd = collect_fvar (collect_app t)._1 in
+      Some (if hd = (`%SH.KSteel ) then ESteel
+       else if hd = (`%SH.KAtomic) then EAtomic
+       else if hd = (`%SH.KGhostI) then EGhostI
+       else if hd = (`%SH.KGhost ) then EGhost
+       else fail "collect_effect_kind")
+    end
+
+let combinable_bind_steel (a0 a1 : Type u#a)
+  : combinable_bind_repr a0 a1 SH.KSteel SH.KSteel SH.KSteel
+  by (norm [delta_attr [`%__repr_M__]])
+  = fun f g -> C.bind f g
+
+let combinable_bind_ghostI (a0 a1 : Type u#a) (opened : Mem.inames)
+  : combinable_bind_repr a0 a1 (SH.KGhostI opened) (SH.KGhostI opened) (SH.KGhostI opened)
+  by (norm [delta_attr [`%__repr_M__]])
+  = fun f g -> C.bind_ek (SH.KGhostI opened) (SH.KGhostI opened) (SH.KGhostI opened)
+      (fun a b f g pre itm post cf cg rf rg -> C.bind_ghostI_steel a b opened f g pre itm post cf cg rf rg)
+      f g
+
+let combinable_bind_atomicL (a0 a1 : Type u#a) (opened : Mem.inames)
+  : combinable_bind_repr a0 a1 (SH.KAtomic opened) (SH.KGhostI opened) (SH.KAtomic opened)
+  by (norm [delta_attr [`%__repr_M__]])
+  = fun f g -> C.bind_ek (SH.KAtomic opened) (SH.KGhostI opened) (SH.KAtomic opened)
+      (fun a b f g pre itm post cf cg rf rg -> C.bind_atomic_ghost_steel a b opened f g pre itm post cf cg rf rg)
+      f g
+
+let combinable_bind_atomicR (a0 a1 : Type u#a) (opened : Mem.inames)
+  : combinable_bind_repr a0 a1 (SH.KGhostI opened) (SH.KAtomic opened) (SH.KAtomic opened)
+  by (norm [delta_attr [`%__repr_M__]])
+  = fun f g -> C.bind_ek (SH.KGhostI opened) (SH.KAtomic opened) (SH.KAtomic opened)
+      (fun a b f g pre itm post cf cg rf rg -> C.bind_ghost_atomic_steel a b opened f g pre itm post cf cg rf rg)
+      f g
+
+let combinable_bind_ghost (a0 a1 : Type u#a) (opened : Mem.inames)
+  : combinable_bind_repr a0 a1 (SH.KGhost opened) (SH.KGhost opened) (SH.KGhost opened)
+  by (norm [delta_attr [`%__repr_M__]])
+  = fun f g -> C.bind_ghost f g
+
+let combinable_bind_op (ek0 ek1 : effect_kind_enum) : term
+  = match if ek0 `ek_le` ek1 then ek1 else ek0 with
+  | EGhost  -> (`combinable_bind_ghost)
+  | EGhostI -> (`combinable_bind_ghostI)
+  | EAtomic -> let ek' = if ek0 `ek_le` ek1 then ek1 else ek0 in
+              if ek' `ek_le` EGhostI
+              then (if ek0 = EAtomic then (`combinable_bind_atomicL) else (`combinable_bind_atomicR))
+              else (`combinable_bind_steel)
+  | ESteel  -> (`combinable_bind_steel)
+
+
+private
+let __build_combinable_ite_t
+      (ek2 : SH.effect_kind{~ (SH.KAtomic? ek2)}) (a : Type) (ek0 ek1 : SH.effect_kind)
+      (lt0 : C.steel_liftable a ek0 ek2) (lt1 : C.steel_liftable a ek1 ek2)
+  = Mkcombinable_ite_t #a #ek0 #ek1 #ek2 () lt0 lt1
+
+let combinable_ite_ghost  o = __build_combinable_ite_t (SH.KGhost  o)
+let combinable_ite_ghostI o = __build_combinable_ite_t (SH.KGhostI o)
+let combinable_ite_steel    = __build_combinable_ite_t  SH.KSteel
+
+let combinable_ite_op (ek0 ek1 : effect_kind_enum) : term
+  = match if ek0 `ek_le` ek1 then ek1 else ek0 with
+  | EGhost  -> (`combinable_ite_ghost)
+  | EGhostI -> (`combinable_ite_ghostI)
+  | EAtomic | ESteel -> (`combinable_ite_steel)
+
+
+/// Try to solves a goal [combinable_bind_t a0 a1 ek0 ek1 ek2] or [combinable_ite_t a ek0 ek1 ek2]:
+/// - succeed and returns true if the heads of ek0 and ek1 are known.
+/// - otherwise, returns false.
+let build_combinable () : Tac bool
+  =
+    let hd, args = collect_app (cur_goal ()) in
+    let hd = try collect_fvar hd with _ -> "unexpected shape" in
+    if hd = (`%combinable_bind_t)
+    then begin
+      guard (L.length args = 5);
+      let ek0 = collect_effect_kind (L.index args 2)._1 in
+      let ek1 = collect_effect_kind (L.index args 3)._1 in
+      match ek0, ek1 with
+      | Some ek0, Some ek1 ->
+             let op = combinable_bind_op ek0 ek1 in
+             apply (`Mkcombinable_bind_t);
+             // cba_bind_repr
+             apply op;
+             // cba_bind_lift0
+             build_steel_liftable ();
+             // cba_bind_lift1
+             build_steel_liftable ();
+             true
+      | _ -> false
+    end else if hd = (`%combinable_ite_t)
+    then begin
+      guard (L.length args = 4);
+      let ek0 = collect_effect_kind (L.index args 1)._1 in
+      let ek1 = collect_effect_kind (L.index args 2)._1 in
+      match ek0, ek1 with
+      | Some ek0, Some ek1 ->
+             let op = combinable_ite_op ek0 ek1 in
+             apply op;
+             // cba_ite_lift0
+             build_steel_liftable ();
+             // cba_ite_lift1
+             build_steel_liftable ();
+             true
+      | _ -> false
+    end else fail "build_combinable : goal_shape"
+
+let rec solve_combinables_round () : Tac (bool & list goal)
+  = match goals () with
+    | [] -> false, []
+    | g :: _ ->
+        if build_combinable ()
+        then
+          let _, gs = solve_combinables_round () in
+          true, gs
+        else begin
+          dismiss ();
+          let b, gs = solve_combinables_round () in
+          b, g :: gs
+        end
+
+let rec solve_combinables () : Tac unit
+  = match goals () with
+  | [] -> ()
+  | _ :: _ ->
+    let b, gs = solve_combinables_round () in
+    if not b then fail "solve_combinables: could not progress";
+    set_goals gs;
+    solve_combinables ()
 
 private
 let __build_mrepr_to_steel_norew
@@ -358,10 +677,10 @@ let __build_mrepr_to_steel_norew
       (goal : (impl : ((pre : M.pre_t) -> (post : M.post_t a) -> (c : M.tree_cond t pre post) ->
                           M.repr_steel_t SH.KSteel a pre post (M.tree_req t c) (M.tree_ens t c))) ->
               ES.__to_steel_goal a pre post req ens M.({repr_tree = t; repr_steel = impl}))
-  : mrepr_to_steel_t flags a pre post req ens t
-  = MReprToSteel (fun r -> goal r.repr_steel)
+  : mrepr_to_steel_t flags a SH.KSteel pre post req ens t
+  = MReprToSteel (fun r -> SH.steel_f (goal r.repr_steel))
 
-/// Solves a goal [mrepr_to_steel_t flags a pre post req ens t] using [ES.build_to_steel].
+/// Solves a goal [mrepr_to_steel_t flags a ek pre post req ens t] using [ES.build_to_steel].
 let build_mrepr_to_steel_norew (fr : flags_record) : Tac unit
   =
     apply (`__build_mrepr_to_steel_norew);
@@ -370,26 +689,43 @@ let build_mrepr_to_steel_norew (fr : flags_record) : Tac unit
     ES.build_to_steel fr
 
 
+inline_for_extraction noextract
+let steel_of_repr_ek
+      (#ek : SH.effect_kind {SH.KSteel? ek \/ SH.KGhost? ek}) // TODO derive for the other effects
+      (#a : Type) (#pre : SE.pre_t) (#post : SE.post_t a) (#req : SE.req_t pre) (#ens : SE.ens_t pre a post)
+      (tr : M.to_repr_t a pre post req ens)
+      (f : M.repr_steel_t ek a tr.r_pre tr.r_post tr.r_req tr.r_ens)
+  : SH.steel a pre post req ens ek
+  = match ek with
+  | SH.KSteel   -> SH.steel_f (M.steel_of_repr tr f)
+  | SH.KGhost o -> SH.ghost_f (M.steel_ghost_of_repr #a #o tr f)
+
 private
 let __build_mrepr_to_steel_wrew
       (flags : list flag)
+      (ek : SH.effect_kind)
       (a : Type) (pre : SE.pre_t) (post : SE.post_t a) (req : SE.req_t pre) (ens : SE.ens_t pre a post)
       (t : prog_tree a)
+      (ek_restr : squash (SH.KSteel? ek \/ SH.KGhost? ek))
       (goal_tr : M.to_repr_t a pre post req ens)
       (goal_sp : ES.to_steel_goal_spec a goal_tr.r_pre goal_tr.r_post goal_tr.r_req goal_tr.r_ens t)
-  : mrepr_to_steel_t flags a pre post req ens t
+  : mrepr_to_steel_t flags a ek pre post req ens t
   = MReprToSteel (fun r ->
-      M.steel_of_repr goal_tr
+      steel_of_repr_ek goal_tr
         (let lc1 = LV.lc_sub_push goal_sp.goal_spec_LV in
          ES.prog_LV_to_Fun_extract_wp r goal_sp.goal_spec_LV lc1 ()
             goal_tr.r_req goal_tr.r_ens (fun sl0 -> goal_sp.goal_spec_WP)))
 
-/// Solves a goal [mrepr_to_steel_t flags a pre post req ens t] using a [rewrite_with_tactic] to avoid
+/// Solves a goal [mrepr_to_steel_t flags a ek pre post req ens t] using a [rewrite_with_tactic] to avoid
 /// normalizing the WP twice.
 let build_mrepr_to_steel_wrew (fr : flags_record) (flags : list flag) : Tac unit
   =
     let fr    = make_flags_record flags in
     apply_raw (`__build_mrepr_to_steel_wrew);
+
+    // ek_restr
+    norm [delta; iota; simplify];
+    trivial ();
 
     // goal_tr
     let t = timer_start "specs     " fr.f_timer in
@@ -402,14 +738,14 @@ let build_mrepr_to_steel_wrew (fr : flags_record) (flags : list flag) : Tac unit
     timer_stop t
 
 
-/// On a goal [mrepr_to_steel_t flags a pre post req ens t] returns [flags].
+/// On a goal [mrepr_to_steel_t flags a ek pre post req ens t] returns [flags].
 let collect_flags () : Tac (list flag)
   =
     let args = (collect_app (cur_goal ()))._2      in
-    guard (L.length args = 7);
+    guard (L.length args = 8);
     unquote (L.hd args)._1
 
-/// Solves a goal [mrepr_to_steel_t flags a pre post req ens t]
+/// Solves a goal [mrepr_to_steel_t flags a ek pre post req ens t].
 let build_mrepr_to_steel () : Tac unit
   =
     let flags = collect_flags ()        in
@@ -422,42 +758,52 @@ let build_mrepr_to_steel () : Tac unit
 [@@ resolve_implicits; __mrepr_implicit__]
 let mrepr_implicits_tac () : Tac unit
   = with_policy Force (fun () ->
-    
-    iterAll (fun () ->
-      intros' ();
-      try first [
-        trefl;
-        (fun () -> apply (`combine_bind));
-        (fun () -> apply (`combine_subcomp_refl));
-        (fun () -> apply (`combine_bind_pure));
-        (fun () -> // if it is an [mrepr_to_steel_t] goal, skip
-                let hd = (collect_app (cur_goal ()))._1 in
-                match inspect hd with
-                | Tv_FVar fv | Tv_UInst fv _ ->
-                  let fv = inspect_fv fv in
-                  guard (implode_qn fv = (`%mrepr_to_steel_t))
-                | _ -> fail "")
-      ] with _ ->
-        // The only sources of Fail_MRepr_implicit should be a bind where the two types involved belong to
-        // different universes. Or a polymonadic bind with an universe greater than [u#8].
-        TcS.cs_raise default_flags TcS.dummy_ctx (fun m -> fail (m Fail_MRepr_implicit [])));
 
-    // At this point there should only remains a [mrepr_to_steel_t] goal
+    //let t = timer_start "implicits" true in
+
+    iterAll (fun () -> intros' (); try trefl () with _ -> ());
+    let fgoals = mrepr_implicits_init (Mkfilter_goals_r [] [] []) in
+
+    // Solve the combinable_* goals
+    set_goals fgoals.fgoals_comb;
+    solve_combinables ();
+
+    // Solve the [steel_liftable] from the lifting to ConvEffect
+    set_goals fgoals.fgoals_lift;
+    iterAll build_steel_liftable;
+
+    //timer_stop t;
+
+    
+    // useful to debug `Tactic left uninstantiated unification variable` errors
+    //dump_all true "implicits";
+
+    // Solve the [mrepr_to_steel_t] goal
+    set_goals fgoals.fgoals_tstl;
     iterAll build_mrepr_to_steel
   )
 
 
-(**** Notations *)
+(*** Notations *)
 
 unfold
-let usteel (a : Type) (pre : SE.pre_t) (post : SE.post_t a)
-          (req : SE.req_t pre) (ens : SE.ens_t pre a post)
-  : Type
-  = SH.unit_steel a pre post req ens
+let usteel = SH.unit_steel
+
+unfold
+let usteel_ghost = SH.unit_steel_ghost
+
 
 let to_steel
       (#[apply (`[])] flags : list flag)
       (#a : Type) (#pre : SE.pre_t) (#post : SE.post_t a) (#req : SE.req_t pre) (#ens : SE.ens_t pre a post)
-      (r : unit -> ConvEffect a pre post req ens flags)
+      (r : unit -> ConvEffect a SH.KSteel pre post req ens flags)
   : usteel a pre post req ens
-  = reify (r ())
+  = SH.steel_u (reify (r ()))
+
+let to_steel_g
+      (#[apply (`[])] flags : list flag)
+      (#a : Type) (#opened : Mem.inames)
+      (#pre : SE.pre_t) (#post : SE.post_t a) (#req : SE.req_t pre) (#ens : SE.ens_t pre a post)
+      (r : unit -> ConvEffect a (SH.KGhost opened) pre post req ens flags)
+  : usteel_ghost a opened pre post req ens
+  = SH.ghost_u (reify (r ()))
